@prefix : <http://vocab.linkeddata.es/datosabiertos/def/medio-ambiente/contaminacion-acustica#> .
@prefix owl: <http://www.w3.org/2002/07/owl#> .
@prefix rdf: <http://www.w3.org/1999/02/22-rdf-syntax-ns#> .
@prefix xml: <http://www.w3.org/XML/1998/namespace> .
@prefix xsd: <http://www.w3.org/2001/XMLSchema#> .
@prefix rdfs: <http://www.w3.org/2000/01/rdf-schema#> .
@base <http://vocab.linkeddata.es/datosabiertos/def/medio-ambiente/contaminacion-acustica> .

<http://vocab.linkeddata.es/datosabiertos/def/medio-ambiente/contaminacion-acustica> rdf:type owl:Ontology ;
                                                                                      owl:imports <http://purl.oclc.org/NET/ssnx/ssn> ,
                                                                                                  <http://vocab.linkeddata.es/datosabiertos/kos/medio-ambiente/contaminacion-acustica> ,
                                                                                                  <http://www.w3.org/2006/time> ;
                                                                                      <http://creativecommons.org/ns#license> "http://creativecommons.org/licenses/by/4.0/" ;
                                                                                      <http://purl.org/dc/elements/1.1/contributor> "Mariano Fernández López (Ontology Engineering Group)"@es ,
                                                                                                                                    "María Poveda Villalón (Ontology Engineering Group)"@es ,
                                                                                                                                    "Oscar Corcho García (Ontology Engineering Group)"@es ,
                                                                                                                                    "Raúl García Castro (Ontology Engineering Group)"@es ;
                                                                                      <http://purl.org/dc/elements/1.1/creator> "Paola Espinoza Arias (Ontology Engineering Group y Secretaría de Educación Superior, Ciencia, Tecnología e Innovación)"@es ;
                                                                                      <http://purl.org/dc/elements/1.1/description> "Este vocabulario extiende la W3C Semantic Sensor Network Ontology (SSN) con clases y propiedades para representar los datos de la contaminación acústica. También se reutiliza la OWL Ontology of Time (OWL-Time)  para representar el tiempo y la WGS84 Geo Positioning Ontology para representar la posición en el espacio a través de la longitud, latitud y altitud"@es ,
                                                                                                                                    "The vocabulary extends W3C Semantic Sensor Network Ontology (SSN) with classes and properties to represent the data about acoustic pollution. Also it reuses OWL-Time Ontology to represent time and WGS84 Geo Positioning Ontology to represent spatial position through longitude, latitude and altitude."@en ;
                                                                                      <http://purl.org/dc/elements/1.1/rights> "Creative Commons Attribution 4.0 International (CC BY 4.0)" ;
                                                                                      <http://purl.org/dc/elements/1.1/title> "Acoustic Pollution"@en ,
                                                                                                                              "Contaminación Acústica"@es .

#################################################################
#    Annotation properties
#################################################################

###  http://purl.org/dc/elements/1.1/contributor
<http://purl.org/dc/elements/1.1/contributor> rdf:type owl:AnnotationProperty .


###  http://purl.org/dc/elements/1.1/description
<http://purl.org/dc/elements/1.1/description> rdf:type owl:AnnotationProperty .


###  http://purl.org/vocab/vann/preferredNamespacePrefix
<http://purl.org/vocab/vann/preferredNamespacePrefix> rdf:type owl:AnnotationProperty .


###  http://purl.org/vocab/vann/preferredNamespaceUri
<http://purl.org/vocab/vann/preferredNamespaceUri> rdf:type owl:AnnotationProperty .


###  http://www.w3.org/1999/02/22-rdf-syntax-ns#value
rdf:value rdf:type owl:AnnotationProperty .


###  http://www.w3.org/2003/01/geo/wgs84_pos#alt
<http://www.w3.org/2003/01/geo/wgs84_pos#alt> rdf:type owl:AnnotationProperty ;
                                              rdfs:comment """The WGS84 altitude of a SpatialThing (decimal meters 
above the local reference ellipsoid).""" ;
                                              rdfs:label "altitude" ;
                                              rdfs:domain <http://www.w3.org/2003/01/geo/wgs84_pos#SpatialThing> .


###  http://www.w3.org/2003/01/geo/wgs84_pos#lat
<http://www.w3.org/2003/01/geo/wgs84_pos#lat> rdf:type owl:AnnotationProperty ;
                                              rdfs:comment "The WGS84 latitude of a SpatialThing (decimal degrees)." ;
                                              rdfs:label "latitude" ;
                                              rdfs:domain <http://www.w3.org/2003/01/geo/wgs84_pos#SpatialThing> .


###  http://www.w3.org/2003/01/geo/wgs84_pos#location
<http://www.w3.org/2003/01/geo/wgs84_pos#location> rdf:type owl:AnnotationProperty ;
                                                   rdfs:subPropertyOf <http://xmlns.com/foaf/0.1/based_near> ;
                                                   rdfs:range <http://www.w3.org/2003/01/geo/wgs84_pos#SpatialThing> .


###  http://www.w3.org/2003/01/geo/wgs84_pos#long
<http://www.w3.org/2003/01/geo/wgs84_pos#long> rdf:type owl:AnnotationProperty ;
                                               rdfs:comment "The WGS84 longitude of a SpatialThing (decimal degrees)." ;
                                               rdfs:label "longitude" ;
                                               rdfs:domain <http://www.w3.org/2003/01/geo/wgs84_pos#SpatialThing> .


###  http://xmlns.com/foaf/0.1/based_near
<http://xmlns.com/foaf/0.1/based_near> rdf:type owl:AnnotationProperty .


#################################################################
#    Object Properties
#################################################################

###  http://purl.oclc.org/NET/ssnx/ssn#observationSamplingTime
<http://purl.oclc.org/NET/ssnx/ssn#observationSamplingTime> rdfs:domain <http://purl.oclc.org/NET/ssnx/ssn#ObservationValue> ;
                                                            rdfs:range <http://www.w3.org/2006/time#TemporalEntity> .


###  http://vocab.linkeddata.es/datosabiertos/def/medio-ambiente/contaminacion-acustica#belongsToSensorClass
:belongsToSensorClass rdf:type owl:ObjectProperty ;
                      rdfs:domain :NoiseSensor ;
                      rdfs:range <http://www.w3.org/2004/02/skos/core#Concept> ;
                      rdfs:comment "El sensor de ruido puede pertenecer o no a una clase. La clase define las caracterísiticas técnicas del sensor que establecen los límites de aceptación y el rango de temperaturas de funcionamiento."@es ,
                                   "Noise sensor may or may not belong to a class. The class defines the technical characteristics of the sensor that establish the limits of acceptance and the range of operating temperatures."@en ;
                      rdfs:label "belongs to sensor class"@en ,
                                 "pertenece a una clase de sensor"@es .


###  http://vocab.linkeddata.es/datosabiertos/def/medio-ambiente/contaminacion-acustica#hasAcousticEmitter
:hasAcousticEmitter rdf:type owl:ObjectProperty ;
                    rdfs:domain :NoiseLevel ;
                    rdfs:range <http://www.w3.org/2004/02/skos/core#Concept> ;
                    rdfs:comment "El nivel de ruido tiene un emisor acústico que lo provoca."@es ,
                                 "Noise level is caused by an acoustic emitter."@en ;
                    rdfs:label "has acoustic emitter"@en ,
                               "tiene emisor acústico"@es .


###  http://vocab.linkeddata.es/datosabiertos/def/medio-ambiente/contaminacion-acustica#hasUnitOfMeasure
:hasUnitOfMeasure rdf:type owl:ObjectProperty ;
                  rdfs:domain <http://purl.oclc.org/NET/ssnx/ssn#SensorOutput> ;
                  rdfs:range <http://www.wurvoc.org/vocabularies/om-1.8/Unit_of_measure> ;
                  rdfs:comment "Relación entre el valor medido por el sensor y  la unidad de medida en la que este valor es expresado."@es ,
                               "Relationship between the measured value by the sensor and the unit of measure of this value."@en ;
                  rdfs:label "has unit of measure"@en ,
                             "tiene unidad de medida"@es .


###  http://vocab.linkeddata.es/datosabiertos/def/medio-ambiente/contaminacion-acustica#isWeightingWith
:isWeightingWith rdf:type owl:ObjectProperty ;
                 rdfs:domain <http://purl.oclc.org/NET/ssnx/ssn#ObservationValue> ;
                 rdfs:range :Weighting ;
                 rdfs:comment "La medida que realiza el Sensor de Ruido tiene una ponderación frecuencial. Puede ser sin poderación (Z), ponderación A o C."@es ,
                              "The measurement performed by the Noise Sensor has a frequency weighting. It can be without weighting (Z), weighting A or C."@en ;
                 rdfs:label "es ponderado con"@es ,
                            "is weighting with"@en .


###  http://vocab.linkeddata.es/datosabiertos/def/medio-ambiente/contaminacion-acustica#lastCalibrationDate
:lastCalibrationDate rdf:type owl:ObjectProperty ;
                     rdfs:domain :NoiseSensor ;
                     rdfs:range <http://www.w3.org/2006/time#Instant> ;
                     rdfs:comment "Last calibration date of the sensor. Calibration is a periodic process performed on acoustic sensors to verify their correct operation in their different working modes."@en ,
                                  "Última fecha de calibración del sensor.  La calibración es un proceso periódico realizado a los sensores acústicos para verificar su correcto funcionamiento en sus distintos modos de trabajo."@es ;
                     rdfs:label "last calibration date"@en ,
                                "última fecha de calibración del sensor."@es .


###  http://vocab.linkeddata.es/datosabiertos/def/medio-ambiente/contaminacion-acustica#referenceInterval
:referenceInterval rdf:type owl:ObjectProperty ;
                   rdfs:domain :NoiseLevel ;
                   rdfs:range <http://www.w3.org/2006/time#TemporalEntity> ;
                   rdfs:comment "Interval of time where the noise assessment was performed. The reference time interval can be specified in national or international standards or by local authorities to encompass typical human activities and variations in the operation of noise sources. The reference time intervals can be for example: a part of the day, a whole day or a complete week. Some countries may even define longer reference intervals."@en ,
                                "Intervalo de tiempo al que se refiere la evaluación del ruido. El intervalo de tiempo de referencia se puede especificar en normas nacionales o internacionales o por las autoridades locales para englobar las actividades humanas típicas y las variaciones en el funcionamiento de las fuentes de ruido. Los intervalos de tiempo de referencia pueden ser por ejemplo: una parte del día, un día entero o una semana completa. Algunos países pueden definir incluso intervalos de referencia más largos."@es ;
                   rdfs:label "intervalo de referencia"@es ,
                              "reference interval"@en ;
                   rdfs:seeAlso "ISO 1996-1: 2005"@es .


###  http://www.w3.org/2003/01/geo/wgs84_pos#location
<http://www.w3.org/2003/01/geo/wgs84_pos#location> rdf:type owl:ObjectProperty .


#################################################################
#    Data properties
#################################################################

###  http://www.co-ode.org/ontologies/ont.owl#timePercentage
<http://www.co-ode.org/ontologies/ont.owl#timePercentage> rdf:type owl:DatatypeProperty ;
                                                          rdfs:domain :PercentilNoiseLevel ;
                                                          rdfs:range xsd:double ;
                                                          rdfs:comment "Percentage of time (N%) of the reference time interval where the noise level is exceeded."@en ,
                                                                       "Porcentaje de tiempo (N%) del intervalo de tiempo de referencia en el que se excede el nivel de ruido."@es ;
                                                          rdfs:label "Porcentaje de tiempo"@es ,
                                                                     "Time percentage"@en .


#################################################################
#    Classes
#################################################################

###  http://vocab.linkeddata.es/datosabiertos/def/medio-ambiente/contaminacion-acustica#AverageNoiseLevel
:AverageNoiseLevel rdf:type owl:Class ;
                   rdfs:subClassOf :NoiseLevel ;
                   rdfs:comment "Average sound pressure level that has been measured by the sensor."@en ,
                                "Nivel medio de presión sonora que ha sido medido por el sensor."@es ;
                   rdfs:label "Average Noise Level"@en ,
                              "Nivel Medio de Ruido"@es .


###  http://vocab.linkeddata.es/datosabiertos/def/medio-ambiente/contaminacion-acustica#NoiseLevel
:NoiseLevel rdf:type owl:Class ;
            rdfs:subClassOf <http://purl.oclc.org/NET/ssnx/ssn#Property> ;
            rdfs:comment "Nivel de presión sonora que ha sido medido por el sensor. Es una magnitud física para describir la contaminación acústica, que tiene relación con los efectos producidos por ésta. Se mide en decibelios (dB)."@es ,
                         "Sound pressure level measured by the sensor. It is a physical magnitude describing acoustic pollution and related to the produced effects. It is measured in decibels (dB)."@en ;
            rdfs:label "Nivel de Ruido"@es ,
                       "Noise Level"@en .


###  http://vocab.linkeddata.es/datosabiertos/def/medio-ambiente/contaminacion-acustica#NoiseSensor
:NoiseSensor rdf:type owl:Class ;
             rdfs:subClassOf <http://purl.oclc.org/NET/ssnx/ssn#SensingDevice> ;
             rdfs:comment "Device that measures the noise level. It detects changes in the air pressure, at a certain location and at a given time, and converts them into electrical pulses. These electric pulses have a frequency, representing the acoustic waves. The frequency range perceived human beings is from 20 Hz to 20 kHz."@en ,
                          "Dispositivo que mide el nivel de ruido. Detecta los cambios en la presión del aire, en determinado lugar y en un momento dado, y los  convierte en pulso eléctricos. Estos pulsos eléctricos tienen una frecuencia, que es la de las ondas acústicas. El rango de frecuencia que percibe el ser humano es de 20 Hz a 20 kHz."@es ;
             rdfs:label "Noise Sensor"@en ,
                        "Sensor de Ruido"@es .


###  http://vocab.linkeddata.es/datosabiertos/def/medio-ambiente/contaminacion-acustica#PercentilNoiseLevel
:PercentilNoiseLevel rdf:type owl:Class ;
                     rdfs:subClassOf :NoiseLevel ;
                     rdfs:comment "Nivel de presión sonora ponderado en frecuencia y ponderado en el tiempo superado el N% de tiempo del intervalo considerado."@es ,
                                  "Weighted frequency and time sound pressure level exceeding the N% of time of the considered interval."@en ;
                     rdfs:label "Nivel de Ruido en Percentiles"@es ,
                                "Percentil Noise Level"@en ;
                     rdfs:seeAlso "AENOR: UNE-ISO 1996-1"@es .


###  http://vocab.linkeddata.es/datosabiertos/def/medio-ambiente/contaminacion-acustica#Weighting
:Weighting rdf:type owl:Class ;
           rdfs:subClassOf <http://www.loa-cnr.it/ontologies/DUL.owl#Method> ;
           rdfs:comment "La medida que realiza el Sensor de Ruido tiene una ponderación frecuencial que se utiliza para una correcta interpretación y medición de  los  niveles  de  sonoridad  de  un  determinado  sonido  en  comparación  con  la naturaleza  no  lineal  del  oído  humano  para  las  distintas  frecuencias  del  espectro audible. Puede ser sin poderación (Z), ponderación A o C."@es ,
                        "The measurement performed by the Noise Sensor has a frequency weighting that is used for a correct interpretation and measurement of the loudness levels of a particular sound compared to the non-linear nature of the human ear for the different frequencies of the audible spectrum. It can be without weighting (Z), weighting A or C."@en ;
           rdfs:label "Ponderación"@es ,
                      "Weighting"@en .


###  http://www.w3.org/2003/01/geo/wgs84_pos#Point
<http://www.w3.org/2003/01/geo/wgs84_pos#Point> rdf:type owl:Class ;
                                                rdfs:subClassOf <http://www.w3.org/2003/01/geo/wgs84_pos#SpatialThing> ;
                                                rdfs:comment """ 
Uniquely identified by lat/long/alt. i.e.

spaciallyIntersects(P1, P2) :- lat(P1, LAT), long(P1, LONG), alt(P1, ALT),
  lat(P2, LAT), long(P2, LONG), alt(P2, ALT).

sameThing(P1, P2) :- type(P1, Point), type(P2, Point), spaciallyIntersects(P1, P2).
  """ ,
                                                             """A point, typically described using a coordinate system relative to Earth, such as WGS84.
  """ ;
                                                rdfs:label "point" .


###  http://www.w3.org/2003/01/geo/wgs84_pos#SpatialThing
<http://www.w3.org/2003/01/geo/wgs84_pos#SpatialThing> rdf:type owl:Class ;
                                                       rdfs:comment """Anything with spatial extent, i.e. size, shape, or position.
 e.g. people, places, bowling balls, as well as abstract areas like cubes.
""" ;
                                                       rdfs:label "SpatialThing" .


###  http://www.w3.org/2004/02/skos/core#Concept
<http://www.w3.org/2004/02/skos/core#Concept> rdf:type owl:Class .


###  http://www.wurvoc.org/vocabularies/om-1.8/Unit_of_measure
<http://www.wurvoc.org/vocabularies/om-1.8/Unit_of_measure> rdf:type owl:Class ;
                                                            rdfs:comment "A unit of measure is a definite magnitude of a quantity, defined and adopted by convention and/or by law. It is used as a standard for measurement of the same quantity, where any other value of the quantity can be expressed as a simple multiple of the unit of measure. For example, length is a quantity; the metre is a unit of length that represents a definite predetermined length. When we say 10 metre (or 10 m), we actually mean 10 times the definite predetermined length called \"metre\"."@en ,
                                                                         "Una unidad de medida es una magnitud definida de una cantidad, definida y adoptada por convención y / o por ley. Se utiliza como estándar para medir la misma cantidad, donde cualquier otro valor de la cantidad puede expresarse como un simple múltiplo de la unidad de medida. Por ejemplo, longitud es una cantidad; El metro es una unidad de longitud que representa una longitud predeterminada definida. Cuando decimos 10 metros (o 10 m), en realidad decimos 10 veces la longitud predeterminada definida llamada \"metro\". (definición tomada de la ontología om)."@es ;
                                                            rdfs:isDefinedBy "http://www.wurvoc.org/vocabularies/om-1.8/" ;
                                                            rdfs:label "Unidad de Medida"@es ,
                                                                       "Unit of Measure"@en .


#################################################################
#    Individuals
#################################################################

###  http://dbpedia.org/resource/Decibel
<http://dbpedia.org/resource/Decibel> rdf:type owl:NamedIndividual ,
                                               <http://www.wurvoc.org/vocabularies/om-1.8/Unit_of_measure> .


###  http://vocab.linkeddata.es/datosabiertos/def/medio-ambiente/contaminacion-acustica#ClaseI
:ClaseI rdf:type owl:NamedIndividual ,
                 <http://www.w3.org/2004/02/skos/core#Concept> ;
        rdfs:comment "Sensor que cumple las características de precisión más restrictivas definidas en la normativa IEC. Esta clase de sensores tiene menores márgenes de tolerancia en su rango de medida. Los instrumentos de Clase I se especifican dentro del rango de temperaturas del aire desde -10 ºC  hasta  +50 ºC."@es ,
                     "Sensor that fulfills the most restrictive precision characteristics defined in the IEC standard. This class of sensors has smaller tolerance margins in its measurement range. Class I instruments are specified within the air temperature range from -10 ° C to +50 ° C."@en ;
        rdfs:label "Clase I"@es ,
                   "Class I"@en ;
        rdfs:seeAlso "Norma IEC 61672-1:2013"@es .


###  http://vocab.linkeddata.es/datosabiertos/def/medio-ambiente/contaminacion-acustica#ClaseII
:ClaseII rdf:type owl:NamedIndividual ,
                  <http://www.w3.org/2004/02/skos/core#Concept> ;
         rdfs:comment "Sensor que cumple las características de precisión menos restrictivas definidas en la normativa IEC. Esta clase de sensores tiene mayores márgenes de tolerancia en su rango de medida. Los instrumentos de Clase II se especifican dentro del rango de temperaturas del aire desde 0 ºC  hasta  +40 ºC."@es ,
                      "Sensor that fulfills the less restrictive precision characteristics defined in the IEC standard. This class of sensors has greater tolerance margins in its measuring range. Class II instruments are specified within the air temperature range from 0 ° C to + 40 ° C."@en ;
         rdfs:label "Clase II"@es ,
                    "Class II"@en ;
         rdfs:seeAlso "Norma IEC 61672-1:2013"@es .


###  http://vocab.linkeddata.es/datosabiertos/def/medio-ambiente/contaminacion-acustica#PonderacionA
:PonderacionA rdf:type owl:NamedIndividual ,
                       :Weighting ,
                       <http://www.w3.org/2004/02/skos/core#Concept> ;
              rdfs:comment "More common weighting in enviromental acoustic. It is used to adjust noise levels as the human ear perceives them."@en ,
                           "Ponderación más habitual en acústica ambiental. Se utiliza para ajustar los niveles de ruido a cómo los percibe el oido humano."@es ;
              rdfs:label "Ponderación A"@es ,
                         "Weighting A"@en ;
              rdfs:seeAlso "Norma IEC 61672:2003"@es .


###  http://vocab.linkeddata.es/datosabiertos/def/medio-ambiente/contaminacion-acustica#PonderacionC
:PonderacionC rdf:type owl:NamedIndividual ,
                       :Weighting ,
                       <http://www.w3.org/2004/02/skos/core#Concept> ;
              rdfs:comment "Ponderación que se utiliza para evaluar altos niveles de ruido."@es ,
                           "Weighting used to evaluate high noise leves."@en ;
              rdfs:label "Ponderación C"@es ,
                         "Weighting C"@en ;
              rdfs:seeAlso "Norma IEC 61672:2003"@es .


###  http://vocab.linkeddata.es/datosabiertos/def/medio-ambiente/contaminacion-acustica#PonderacionZ
:PonderacionZ rdf:type owl:NamedIndividual ,
                       :Weighting ,
                       <http://www.w3.org/2004/02/skos/core#Concept> ;
              rdfs:comment "It represents the fact of not applying any type of frequency weighting to the sound waves captured by the noise sensor. They are captured as they are."@en ,
                           "Representa el hecho de no aplicar ningún tipo de ponderación frecuencial a las ondas sonoras captadas por el sensor de ruido. Se captan tal y como son."@es ;
              rdfs:label "Ponderación Z"@es ,
                         "Weighting Z"@en ;
              rdfs:seeAlso "Norma IEC 61672:2003"@es .


#################################################################
#    Annotations
#################################################################

<http://www.w3.org/2003/01/geo/wgs84_pos#> <http://purl.org/dc/elements/1.1/date> "$Date: 2009/04/20 15:00:30 $" ;
                                           <http://purl.org/dc/elements/1.1/description> """A vocabulary for representing latitude, longitude and 
 altitude information in the WGS84 geodetic reference datum. 
 Version $Id: wgs84_pos.rdf,v 1.22 2009/04/20 15:00:30 timbl Exp $. See http://www.w3.org/2003/01/geo/ for more details.""" ;
                                           <http://purl.org/dc/elements/1.1/title> "WGS84 Geo Positioning: an RDF vocabulary" ;
                                           rdfs:comment """
Recent changes to this namespace:
$Log: wgs84_pos.rdf,v $
Revision 1.22  2009/04/20 15:00:30  timbl
Remove the time bits which have been deal with elsewhere eg in iCal.

Revision 1.21  2009/04/20 12:52:47  timbl
try again

Revision 1.20  2009/04/20 12:42:11  timbl
Add Event (edited ages ago and never checked in), and location (following discussion http://chatlogs.planetrdf.com/swig/2009-04-20#T12-36-09)

Revision 1.19  2009/04/20 12:36:31  timbl
Add Event (edited ages ago and never checked in), and location (following discussion http://chatlogs.planetrdf.com/swig/2009-04-20#T12-36-09)

Revision 1.18  2006/02/01 22:01:04  danbri
Clarified that lat and long are decimal degrees, and that alt is decimal metres about local reference ellipsoid

Revision 1.17  2004/02/06 17:38:12  danbri
Fixed a bad commit screwup

Revision 1.15  2003/04/19 11:24:08  danbri
Fixed the typo even more.

Revision 1.14  2003/04/19 11:16:56  danbri
fixed a typo

Revision 1.13  2003/02/19 22:27:27  connolly
relaxed domain constraints on lat/long/alt from Point to SpatialThing

Revision 1.12  2003/01/12 01:41:41  danbri
Trying local copy of XSLT doc.

Revision 1.11  2003/01/12 01:20:18  danbri
added a link to morten's xslt rdfs viewer.

Revision 1.10  2003/01/11 18:56:49  danbri
Removed datatype range from lat and long properties, since they would
have required each occurance of the property to mention the datatype.

Revision 1.9  2003/01/11 11:41:31  danbri
Another typo; repaired rdfs:Property to rdf:Property x4

Revision 1.8  2003/01/11 11:05:02  danbri
Added an rdfs:range for each lat/long/alt property,
http://www.w3.org/2001/XMLSchema#float

Revision 1.7  2003/01/10 20:25:16  danbri
Longer rdfs:comment for Point, trying to be Earth-centric and neutral about
coordinate system(s) at the same time. Feedback welcomed.

Revision 1.6  2003/01/10 20:18:30  danbri
Added CVS log comments into the RDF/XML as an rdfs:comment property of the
vocabulary. Note that this is not common practice (but seems both harmless
and potentially useful).


revision 1.5
date: 2003/01/10 20:14:31;  author: danbri;  state: Exp;  lines: +16 -5
Updated schema:
Added a dc:date, added url for more info. Changed the rdfs:label of the
namespace from gp to geo. Added a class Point, set as the rdfs:domain of
each property. Added XML comment on the lat_long property suggesting that
we might not need it (based on #rdfig commentary from implementors).

revision 1.4
date: 2003/01/10 20:01:07;  author: danbri;  state: Exp;  lines: +6 -5
Fixed typo; several rdfs:about attributes are now rdf:about. Thanks to MortenF in
#rdfig for catching this error.

revision 1.3
date: 2003/01/10 11:59:03;  author: danbri;  state: Exp;  lines: +4 -3
fixed buglet in vocab, added more wgs links

revision 1.2
date: 2003/01/10 11:01:11;  author: danbri;  state: Exp;  lines: +4 -4
Removed alt from the as-a-flat-string property, and switched from
space separated to comma separated.

revision 1.1
date: 2003/01/10 10:53:23;  author: danbri;  state: Exp;
basic geo vocab

""" ;
                                           rdfs:label "geo" .


<http://www.w3.org/2003/01/geo/wgs84_pos#lat_long> rdfs:comment "A comma-separated representation of a latitude, longitude coordinate." ;
                                                   rdfs:label "lat/long" .


<http://www.w3.org/2003/01/geo/wgs84_pos#location> rdfs:comment """The relation between something and the point, 
 or other geometrical thing in space, where it is.  For example, the realtionship between
 a radio tower and a Point with a given lat and long.
 Or a relationship between a park and its outline as a closed arc of points, or a road and
 its location as a arc (a sequence of points).
 Clearly in practice there will be limit to the accuracy of any such statement, but one would expect
 an accuracy appropriate for the size of the object and uses such as mapping .
 """ ;
                                                   rdfs:label "location" .


###  Generated by the OWL API (version 5.1.11) https://github.com/owlcs/owlapi/
